Update coq files

exercises/exercise3-01.v
@@ -2,78 +2,78 @@ Require Import List.
 
 Import ListNotations.
 
-Inductive aExpr :=
-| Num : nat -> aExpr
-| Plus : aExpr -> aExpr -> aExpr
-| Mult : aExpr -> aExpr -> aExpr
+Inductive a_expr :=
+| Num : nat -> a_expr
+| Plus : a_expr -> a_expr -> a_expr
+| Mult : a_expr -> a_expr -> a_expr
 .
 
-Fixpoint aInterpret (e : aExpr) : nat :=
+Fixpoint a_interpret (e : a_expr) : nat :=
   match e with
   | Num n => n
-  | Plus e1 e2 => aInterpret e1 + aInterpret e2
-  | Mult e1 e2 => aInterpret e1 * aInterpret e2
+  | Plus e1 e2 => a_interpret e1 + a_interpret e2
+  | Mult e1 e2 => a_interpret e1 * a_interpret e2
   end
 .
 
-Inductive aInstruction :=
-| INum : nat -> aInstruction
-| IPlus : aInstruction
-| IMult : aInstruction
+Inductive a_instruction :=
+| INum : nat -> a_instruction
+| IPlus : a_instruction
+| IMult : a_instruction
 .
 
-Fixpoint aEval' (aIs : list aInstruction) (stk : list nat) : option nat :=
-  match aIs with
+Fixpoint a_eval' (a_is : list a_instruction) (stk : list nat) : option nat :=
+  match a_is with
   | [] =>
     match stk with
     | [n] => Some n
     | _ => None
     end
-  | INum n :: aIs' => aEval' aIs' (n :: stk)
-  | IPlus :: aIs' =>
+  | INum n :: a_is' => a_eval' a_is' (n :: stk)
+  | IPlus :: a_is' =>
     match stk with
-    | n0 :: n1 :: stk' => aEval' aIs' (n1 + n0 :: stk')
+    | n0 :: n1 :: stk' => a_eval' a_is' (n1 + n0 :: stk')
     | _ => None
     end
-  | IMult :: aIs' =>
+  | IMult :: a_is' =>
     match stk with
-    | n0 :: n1 :: stk' => aEval' aIs' (n1 * n0 :: stk')
+    | n0 :: n1 :: stk' => a_eval' a_is' (n1 * n0 :: stk')
     | _ => None
     end
   end.
 
-Definition aEval (state : list aInstruction * list nat) : option nat :=
+Definition a_eval (state : list a_instruction * list nat) : option nat :=
   match state with
-  | (aIs, stk) => aEval' aIs stk
+  | (a_is, stk) => a_eval' a_is stk
   end
 .
 
-Fixpoint aCompile (e : aExpr) : list aInstruction :=
+Fixpoint a_compile (e : a_expr) : list a_instruction :=
   match e with
   | Num n => [INum n]
-  | Plus e1 e2 => aCompile e1 ++ aCompile e2 ++ [IPlus]
-  | Mult e1 e2 => aCompile e1 ++ aCompile e2 ++ [IMult]
+  | Plus e1 e2 => a_compile e1 ++ a_compile e2 ++ [IPlus]
+  | Mult e1 e2 => a_compile e1 ++ a_compile e2 ++ [IMult]
   end
 .
 
-Lemma interpret_compile_equiv_general : forall (aIs : list aInstruction) (stk : list nat) (e : aExpr),
-    aEval (aIs, aInterpret e :: stk) = aEval (aCompile e ++ aIs, stk)
+Lemma interpret_compile_equiv_general : forall (a_is : list a_instruction) (stk : list nat) (e : a_expr),
+    a_eval (a_is, a_interpret e :: stk) = a_eval (a_compile e ++ a_is, stk)
 .
 Proof.
-  intros; generalize dependent stk; generalize dependent aIs.
+  intros; generalize dependent stk; generalize dependent a_is.
   induction e; intros; simpl; auto; try (
     repeat rewrite app_assoc_reverse;
-    unfold aEval in IHe1; unfold aEval in IHe2;
+    unfold a_eval in IHe1; unfold a_eval in IHe2;
     rewrite <- IHe1; rewrite <- IHe2; now auto
   ).
 Qed.
 
-Theorem interpret_compile_equiv : forall (e : aExpr),
-    Some (aInterpret e) = aEval (aCompile e, [])
+Theorem interpret_compile_equiv : forall (e : a_expr),
+    Some (a_interpret e) = a_eval (a_compile e, [])
 .
 Proof.
   intros.
-  replace (aCompile e) with (aCompile e ++ []);
+  replace (a_compile e) with (a_compile e ++ []);
     auto with datatypes.
   rewrite <- interpret_compile_equiv_general.
   now auto.
